LibDecomp.v
@@ -1,0 +1,56 @@
+(** ** Specific redefinition of usual tactics. *)
+
+(** Note that for example !!induction h doesn not work because
+    "destruct" is not a ltac function by itself, it is already a
+    notation. Hence the special definitions below for this kind of
+    tactics: induction ddestruct inversion etc. *)
+
+Ltac decomp_logicals h :=
+  match type of h with
+  | @ex _ (fun x => _) => let x' := fresh x in let h1 := fresh in destruct h as [x' h1]; decomp_logicals h1
+  | @sig _ (fun x => _) => let x' := fresh x in let h1 := fresh in destruct h as [x' h1]; decomp_logicals h1
+  | @sig2 _ (fun x => _) (fun _ => _) => let x' := fresh x in
+                                         let h1 := fresh in 
+                                         let h2 := fresh in
+                                         destruct h as [x' h1 h2];
+                                         decomp_logicals h1;
+                                         decomp_logicals h2
+  | @sigT _ (fun x => _) => let x' := fresh x in let h1 := fresh in destruct h as [x' h1]; decomp_logicals h1
+  | @sigT2 _ (fun x => _) (fun _ => _) => let x' := fresh x in
+                                          let h1 := fresh in
+                                          let h2 := fresh in
+                                          destruct h as [x' h1 h2]; decomp_logicals h1; decomp_logicals h2
+  | and _ _ => let h1 := fresh in let h2 := fresh in destruct h as [h1 h2]; decomp_logicals h1; decomp_logicals h2
+  | or _ _ => let h' := fresh in destruct h as [h' | h']; [decomp_logicals h' | decomp_logicals h' ]
+  | _ => idtac
+  end.
+
+(* decompose and ex and or at once. TODO: generalize. *)
+(* clear may fail if h is not a hypname *)
+(* Tactic Notation "decomp" hyp(h) :=
+   (!! (idtac;decomp_logicals h)). *) (* Why do I need this idtac? Without it no rename happens. *)
+
+Ltac decompose_clear c :=
+  let h := fresh "h_decomp" in
+  pose proof c as h;
+  decomp_logicals c; try clear h.
+(*
+Lemma foo : forall x, { aa:nat | (aa = x /\ x=aa) & (aa = aa /\ aa= x) } -> False.
+Proof.
+  intros x H. 
+  decomp H.
+Abort.
+
+Lemma foo : { aa:False & True  } -> False.
+Proof.
+  intros H. 
+  decomp H.
+Abort.
+
+
+Lemma foo : { aa:False & True & False  } -> False.
+Proof.
+  intros H. 
+  decomp H.
+Abort.
+*)
