LibTac.v
@@ -1,0 +1,49 @@
+Require Import TacNewHyps.
+Require Import LibHypsNaming.
+Require Import LibDecomp.
+Tactic Notation "decomp" constr(c) := (!!decompose_clear c).
+(*
+Lemma foo : forall x, { aa:nat | (aa = x /\ x=aa) & (aa = aa /\ aa= x) } -> False.
+Proof.
+  intros x H. 
+  decomp H.
+Abort.
+
+Lemma foo : { aa:False & True  } -> False.
+Proof.
+  intros H. 
+  decomp H.
+Abort.
+
+
+Lemma foo : { aa:False & True & False  } -> False.
+Proof.
+  intros H. 
+  decomp H.
+Abort.
+*)
+  
+(** Some more tactic not specially dedicated to renaming. *)
+
+(* This performs the map from "top" to "bottom" (from older to younger hyps). *)
+Ltac map_hyps_rev tac hs :=
+  idtac;
+  let rec step H hs := tac H ; next_hyp hs step idtac in
+  next_hyp hs step idtac.
+
+Ltac map_all_hyps tac := map_hyps tac all_hyps.
+Ltac map_all_hyps_rev tac := map_hyps_rev tac all_hyps.
+
+(* A tactic which moves up a hypothesis if it sort is Type or Set. *)
+Ltac move_up_types H := match type of H with
+                        | ?T => match type of T with
+                                | Prop => idtac
+                                | Set => move H at top
+                                | Type => move H at top
+                                end
+                        end.
+
+(* Iterating the tactic on all hypothesis. Moves up all Set/Type
+   variables to the top. Really useful with [Set Compact Context]
+   which is no yet commited in coq-trunk. *)
+Ltac up_type := map_all_hyps_rev move_up_types.
